LinearAlgebraInLean/VectorSpace/FundamentalTheoremOnHomomorphisms.lean
@@ -13,8 +13,11 @@ variable {U : Subspace V}
 def InducedMap (Φ: LinearMap V W) : LinearMap (V / (Kernel.kernel Φ)) W := by
 
   let Φt : V / (Kernel.kernel Φ) -> W := Quotient.lift (fun x => Φ x) <| by
+    -- some proof for a ≈ b → (fun x => Φ x) a = (fun x => Φ x) b
     intro a b hab
     simp
+    --have : a - b ∈  Kernel.kernel Φ := by assumption
+
     simp[HasEquiv.Equiv, instHasEquivOfSetoid] at hab
     unfold Setoid.r QuotientSpace.rel at hab
     unfold QuotientSpace.relation at hab
@@ -28,7 +31,7 @@ def InducedMap (Φ: LinearMap V W) : LinearMap (V / (Kernel.kernel Φ)) W := by
   induction u using Quotient.ind
   rename_i v u
 
-  let mk x := Quotient.mk (QuotientSpace.rel V (Kernel.kernel Φ)) x
+  let mk x : (V / (Kernel.kernel Φ)) := QuotientSpace.mk x
 
   exact calc
     Φt (μ • mk v + mk u)
@@ -36,27 +39,25 @@ def InducedMap (Φ: LinearMap V W) : LinearMap (V / (Kernel.kernel Φ)) W := by
     _ = μ • Φ v + Φ u := by simp
     _ = μ • (Φt (mk v)) + Φt (mk u) := by rfl
 
-theorem inducedMapIsInjective (Φ: LinearMap V W) : Function.Injective (InducedMap Φ) := by
+theorem inducedMapIsInjective (Φ: LinearMap V W) :
+    Function.Injective (InducedMap Φ) := by
   unfold Function.Injective
   intro a b h
   induction a using Quotient.ind
   induction b using Quotient.ind
   rename_i a b
 
-  let mk x := Quotient.mk (QuotientSpace.rel V (Kernel.kernel Φ)) x
-
-  have : Φ a = Φ b := calc
+  let mk x : (V / (Kernel.kernel Φ)) := QuotientSpace.mk x
+  have : Φ a = Φ b := by calc
     Φ a
     _ = (InducedMap Φ).hom (mk a) := by rfl
     _ = (InducedMap Φ).hom (mk b) := by exact h
     _ = Φ b := by rfl
 
   have : a - b ∈ Kernel.kernel Φ := Image.in_kernel_from_same_image this
+
   apply Quotient.sound
-  simp[HasEquiv.Equiv, instHasEquivOfSetoid]
-  unfold Setoid.r QuotientSpace.rel
-  unfold QuotientSpace.relation
-  simp
+  have : QuotientSpace.relation V (Kernel.kernel Φ) a b := by assumption
   assumption
 
 theorem originalIsInduedAndProjection (φ: LinearMap V W) : φ = (InducedMap φ) ∘ QuotientSpace.π := by
@@ -64,3 +65,9 @@ theorem originalIsInduedAndProjection (φ: LinearMap V W) : φ = (InducedMap φ)
   intro x
   simp [chain, Function.comp]
   rfl
+
+theorem inducedMapIsSurjective {Φ: LinearMap V W} (h: Function.Surjective Φ) : Function.Surjective (InducedMap Φ) := by
+  unfold Function.Surjective x
+  intro b
+  have ⟨a,ha⟩ := h b
+  exists QuotientSpace.π a
